Expr.v
@@ -102,12 +102,12 @@ Module SmokeTest.
 
   Lemma nat_always : 
     forall (n : nat) (s : state Z), [| Nat n |] s => (Z.of_nat n).
-  Proof. admit. Qed.
+  Proof. admit. Admitted.
 
   Lemma double_and_sum : 
     forall (s : state Z) (e : expr) (z : Z), 
       [| e [*] (Nat 2) |] s => z -> [| e [+] e |] s => z.
-  Proof. admit. Qed.
+  Proof. admit. Admitted.
 
 End SmokeTest.
 
@@ -136,19 +136,19 @@ where "x ? e" := (V e x).
 *)
 Lemma defined_expression: forall (e : expr) (s : state Z) (z : Z) (id : id),
   [| e |] s => z -> id ? e -> exists z', s / id => z'.
-Proof. admit. Qed.
+Proof. admit. Admitted.
 
 (* If a variable in expression is undefined in some state, then the expression
    is undefined is that state as well
 *)
 Lemma undefined_variable: forall (e : expr) (s : state Z) (id : id),
   id ? e -> (forall (z : Z), ~ (s / id => z)) -> (forall (z : Z), ~ ([| e |] s => z)).
-Proof. admit. Qed.
+Proof. admit. Admitted.
 
 (* The evaluation relation is deterministic *)
 Lemma bs_eval_deterministic: forall (e : expr) (s : state Z) (z1 z2 : Z),
   [| e |] s => z1 -> [| e |] s => z2 -> z1 = z2.
-Proof. admit. Qed.
+Proof. admit. Admitted.
 
 (* Equivalence of states w.r.t. an identifier *)
 Definition equivalent_states (s1 s2 : state Z) (id : id) :=
@@ -160,7 +160,122 @@ Definition equivalent_states (s1 s2 : state Z) (id : id) :=
 Lemma variable_relevance: forall (e : expr) (s1 s2 : state Z) (z : Z),
   (forall (id : id) (z : Z), id ? e -> equivalent_states s1 s2 id) -> 
   [| e |] s1 => z -> [| e |] s2 => z.
-Proof. admit. Qed.
+Proof. admit. Admitted.
+
+(* Semantic equivalence *)
+Reserved Notation "e1 '~~' e2" (at level 42, no associativity).
+
+Inductive equivalent: expr -> expr -> Prop := 
+  eq_intro : forall (e1 e2 : expr), 
+               (forall (n : Z) (s : state Z), 
+                 [| e1 |] s => n <-> [| e2 |] s => n
+               ) -> e1 ~~ e2
+where "e1 '~~' e2" := (equivalent e1 e2).
+
+(* Semantic equivalence is an equivalence relation *)
+Lemma eq_refl: forall (e : expr), e ~~ e.
+Proof. admit. Admitted.
+
+Lemma eq_symm: forall (e1 e2 : expr), e1 ~~ e2 -> e2 ~~ e1.
+Proof. admit. Admitted.
+
+Lemma eq_trans: forall (e1 e2 e3 : expr), e1 ~~ e2 -> e2 ~~ e3 -> e1 ~~ e3.
+Proof. admit. Admitted.
+ 
+(* Contexts *)
+Inductive Context : Type :=
+  | Hole : Context
+  | AddL : Context -> expr -> Context
+  | SubL : Context -> expr -> Context
+  | MulL : Context -> expr -> Context
+  | DivL : Context -> expr -> Context
+  | ModL : Context -> expr -> Context
+  | LeL  : Context -> expr -> Context
+  | LtL  : Context -> expr -> Context
+  | GeL  : Context -> expr -> Context
+  | GtL  : Context -> expr -> Context
+  | EqL  : Context -> expr -> Context
+  | NeL  : Context -> expr -> Context
+  | AndL : Context -> expr -> Context
+  | OrL  : Context -> expr -> Context
+  | AddR : expr -> Context -> Context
+  | SubR : expr -> Context -> Context
+  | MulR : expr -> Context -> Context
+  | DivR : expr -> Context -> Context
+  | ModR : expr -> Context -> Context
+  | LeR  : expr -> Context -> Context
+  | LtR  : expr -> Context -> Context
+  | GeR  : expr -> Context -> Context
+  | GtR  : expr -> Context -> Context
+  | EqR  : expr -> Context -> Context
+  | NeR  : expr -> Context -> Context
+  | AndR : expr -> Context -> Context
+  | OrR  : expr -> Context -> Context.
+
+(* Plugging an expression into a context *)
+Fixpoint plug (C : Context) (e : expr) : expr := 
+  match C with
+  | Hole => e
+  | AddL C e1 => Add (plug C e) e1
+  | SubL C e1 => Sub (plug C e) e1
+  | MulL C e1 => Mul (plug C e) e1
+  | DivL C e1 => Div (plug C e) e1
+  | ModL C e1 => Mod (plug C e) e1
+  | LeL  C e1 => Le  (plug C e) e1
+  | LtL  C e1 => Lt  (plug C e) e1
+  | GeL  C e1 => Ge  (plug C e) e1
+  | GtL  C e1 => Gt  (plug C e) e1
+  | EqL  C e1 => Eq  (plug C e) e1
+  | NeL  C e1 => Ne  (plug C e) e1
+  | AndL C e1 => And (plug C e) e1
+  | OrL  C e1 => Or  (plug C e) e1
+  | AddR e1 C => Add e1 (plug C e)
+  | SubR e1 C => Sub e1 (plug C e)
+  | MulR e1 C => Mul e1 (plug C e)
+  | DivR e1 C => Div e1 (plug C e)
+  | ModR e1 C => Mod e1 (plug C e)
+  | LeR  e1 C => Le  e1 (plug C e)
+  | LtR  e1 C => Lt  e1 (plug C e)
+  | GeR  e1 C => Ge  e1 (plug C e)
+  | GtR  e1 C => Gt  e1 (plug C e)
+  | EqR  e1 C => Eq  e1 (plug C e)
+  | NeR  e1 C => Ne  e1 (plug C e)
+  | AndR e1 C => And e1 (plug C e)
+  | OrR  e1 C => Or  e1 (plug C e)
+  end.  
+
+Notation "C '<~' e" := (plug C e) (at level 43, no associativity).
+
+(* Contextual equivalence *)
+Reserved Notation "e1 '~c~' e2" (at level 42, no associativity).
+
+Inductive contextual_equivalent: expr -> expr -> Prop :=
+  ceq_intro : forall (e1 e2 : expr),
+                (forall (C : Context), (C <~ e1) ~~ (C <~ e2)) -> e1 ~c~ e2
+where "e1 '~c~' e2" := (contextual_equivalent e1 e2).
+
+(* Contextual equivalence is equivalent to the semantic one *)
+Lemma eq_eq_ceq: forall (e1 e2 : expr), e1 ~~ e2 <-> e1 ~c~ e2.
+Proof. admit. Admitted.
+
+
+
+
+
+
+
+
+
+
+
+
+
+
+
+
+
+
+
 
  
 
