Id.v
@@ -27,38 +27,38 @@ Notation "n >>  m" := (gt_id n m).
 Notation "n <<  m" := (lt_id n m).
 
 Lemma lt_eq_lt_id_dec: forall (id1 id2 : id), {id1 << id2} + {id1 = id2} + {id2 << id1}.
-Proof. admit. Qed.
+Proof. admit. Admitted.
 
 Lemma gt_eq_gt_id_dec: forall (id1 id2 : id), {id1 >> id2} + {id1 = id2} + {id2 >> id1}.
-Proof. admit. Qed.
+Proof. admit. Admitted.
 
 Lemma le_gt_id_dec : forall id1 id2 : id, {id1 <<= id2} + {id1 >> id2}.
-Proof. admit. Qed.
+Proof. admit. Admitted.
 
 Lemma eq_dec : forall n m : nat, {n = m} + {n <> m}.
-Proof. admit. Qed.
+Proof. admit. Admitted.
 
 Lemma eq_id_dec : forall id1 id2 : id, {id1 = id2} + {id1 <> id2}.
-Proof. admit. Qed. 
+Proof. admit. Admitted. 
 
 Lemma eq_id : forall (T:Type) x (p q:T), (if eq_id_dec x x then p else q) = p. 
-Proof. admit. Qed.
+Proof. admit. Admitted.
 
 Lemma neq_id : forall (T:Type) x y (p q:T), x <> y -> (if eq_id_dec x y then p else q) = q. 
-Proof. admit. Qed.
+Proof. admit. Admitted.
 
 Lemma lt_gt_id_false : forall id1 id2 : id, id1 >> id2 -> id2 >> id1 -> False.
-Proof. admit. Qed.
+Proof. admit. Admitted.
 
 Lemma le_gt_id_false : forall id1 id2 : id, id2 <<= id1 -> id2 >> id1 -> False.
-Proof. admit. Qed.
+Proof. admit. Admitted.
 
 Lemma le_lt_eq_id_dec : forall id1 id2 : id, id1 <<= id2 -> {id1 = id2} + {id2 >> id1}.
-Proof. admit. Qed.
+Proof. admit. Admitted.
 
 Lemma neq_lt_gt_id_dec : forall id1 id2 : id, id1 <> id2 -> {id1 >> id2} + {id2 >> id1}.
-Proof. admit. Qed.
+Proof. admit. Admitted.
     
 Lemma eq_gt_id_false : forall id1 id2 : id, id1 = id2 -> id1 >> id2 -> False.
-Proof. admit. Qed.
+Proof. admit. Admitted.
 
