State.v
@@ -25,28 +25,28 @@ Section S.
 
   Lemma state_deterministic: forall (st : state) (x : id) (n m : A),
     st / x => n -> st / x => m -> n = m.
-  Proof. admit. Qed.    
+  Proof. admit. Admitted.    
 
   Lemma update_eq : forall (st : state) (x : id) (n : A),
     st [x <- n] / x => n.
-  Proof. admit. Qed.
+  Proof. admit. Admitted.
 
   Lemma update_neq : forall (st : state) (x2 x1 : id) (n m : A),
     x2 <> x1 -> st / x1 => m -> st [x2 <- n] / x1 => m.
-  Proof. admit. Qed.
+  Proof. admit. Admitted.
 
   Lemma update_shadow : forall (st : state) (x1 x2 : id) (n1 n2 m : A),
     st[x2 <- n1][x2 <- n2] / x1 => m -> st[x2 <- n2] / x1 => m.
-  Proof. admit. Qed.
+  Proof. admit. Admitted.
 
   Lemma update_same : forall (st : state) (x1 x2 : id) (n1 m : A),
     st / x1 => n1 -> st / x2 => m -> st [x1 <- n1] / x2 => m.
-  Proof. admit. Qed.
+  Proof. admit. Admitted.
 
   Lemma update_permute : forall (st : state) (x1 x2 x3 : id) (n1 n2 m : A),
     x2 <> x1 -> 
     st [x2 <- n1][x1 <- n2] / x3 => m ->
     st [x1 <- n2][x2 <- n1] / x3 => m.
-  Proof. admit. Qed.  
+  Proof. admit. Admitted.  
 
 End S.
